# Let $f$ be continuous. Prove that $f$ may be written as $f(x) = $g(x) - h(x)$, for some continuous functions $g$ and $h$ which are also nonnegative (meaning $g(x) > 0$ and $h(x) > 0$ for all $x$).

Define:

$$
g(x)=\begin{cases}
    f(x) \quad &\text{if} \quad f(x) > 0\\
    0 \quad &\text{if} \quad f(x) \leq 0
\end{cases}
$$

$$
h(x)=\begin{cases}
    -f(x) \quad &\text{if} \quad f(x) < 0\\
    0 \quad &\text{if} \quad f(x) \geq 0
\end{cases}
$$

Then clearly $f(x)=g(x)-h(x)$. Note as well that both are nonnegative. It remains to show that they are continuous, which we'll prove only $g$, since the reasoning for $h$ is pretty much the same.

Let $c \in \mathbb R$. Let $\epsilon \leq \frac{|f(c)|}{2}$. 

By continuity of $f$, there is $\delta_\epsilon > 0$ such that $x\in(c-\delta_\epsilon,c+\delta_\epsilon) \implies f(x) \in (f(c)-\epsilon,f(c)+\epsilon)$

If $f(c) > 0$, then for every $x\in(c-\delta_\epsilon,c+\delta_\epsilon)$ it follows that $(f(c)-\epsilon,f(c)+\epsilon) \subset (0,+\infty)$, which implies that for such $x$`s, $g(x)=f(x)$ and $g(c)=f(c)$, so it follows that $|g(x)-g(c)|=|f(x)-f(c)|<\epsilon$.

If $f(c) \leq 0$, then for every $x\in(c-\delta_\epsilon,c+\delta_\epsilon)$ it follows that $(f(c)-\epsilon,f(c)+\epsilon) \subset (-\infty,0)$, which implies that for such $x$`s, $g(x)=0$ and $g(c)=0$, so it follows that $|g(x)-g(c)| = 0 <\epsilon$.

### Final note
For any $\epsilon > \frac{|f(c)|}{2}$, any given $\delta_\epsilon$ from continuity of $f$ and $\epsilon \leq \frac{|f(c)|}{2}$ is sufficient.

