# In this exercise you will prove the *Banach fixed-point theorem*. Let $f:\mathbb R \rightarrow \mathbb R$, and assume there exists some $0< C < 1$ such that $\left|f(x)-f(y)\right|<C\left|x-y\right|$ for all $x,y \in \mathbb R$ (such functions are called *Lipschitz*).

## a) Prove that $f$ is continuous on $\mathbb R$.

## b) Pick any $x_1\in\mathbb R$ and consider the sequence where, for $n>1$, we have $x_n = f(x_{n-1})$. That is, this is the sequence $(x_1,f(x_1),f(f(x_1)),f(f(f(x_1))),\cdots)$. Prove that this sequence converges by showing it is Cauchy.

## c) Let $x = \lim_{x\to\infty} x_n$. Prove that $x$ is a fixed point. That is, prove that $f(x)=x$.

## d) Prove that this $x$ is the only fixed point of $f$.

a) We start by showing that $f$ is continuous on $\mathbb R$. For that purpose, let $c \in \mathbb R$ and $\epsilon > 0$. We aim to find $\delta > 0$ such that $|x-c| < \delta \implies |f(x)-f(c)| < \epsilon$.

We already know that for any $x,y \in \mathbb R$, we have a constant $C < 1$ such that $|f(x)-f(y)| \leq C|x-y|$, so all we need to do to find such $\delta$ is to set it to be equal to $\epsilon$, because if $|x-y|<\epsilon$, then $|f(x)-f(y)| \leq  C|x-y| < C\epsilon < \epsilon$, as desired.

---
b) We want to show the convergence of that sequence by showing it is Cauchy. For that purpose, lets study the distance between any two terms of the sequence, namely $x_n, x_m$. Suppose, wlog, that $n<m$, therefore:

$$
\begin{align*}
    |x_m-x_n| &= |f(x_{m-1})-f(x_{n-1})|\\
    &\leq C|x_{m-1}-x_{n-1}|\\
    &\leq C^2|x_{m-2} - x_{n-2}|\\
    &\vdots\\
    &\leq C^{n}|x_{m-n} - x_0|
\end{align*}
$$

Note as well that 

$$
\begin{align*}
    |x_{m-n} - x_0| &< |x_{m-n} - x_{m-n-1}| + |x_{m-n-1} - x_{m-n-2}| + \cdots + |x_1 - x_0|\\
    &\leq  C^{m-n}|x_1 - x_0| + C^{m-n-1}|x_1 - x_0| + \cdots + |x_1-x_0|\\
    &= (C^{m-n} + C^{m-n-1} + \cdots + 1)|x_1-x_0|
\end{align*}
$$

Therefore

$$
\begin{align*}
    |x_m-x_n| & \leq  C^{n}\bigg((C^{m-n} + C^{m-n-1} + \cdots + 1)|x_1-x_0|\bigg)\\
    & \leq  (C^{m} + C^{m-1} + \cdots + C^n)|x_1-x_0|\\
    &= C^n\frac{1-C^{m+1}}{1-C}|x_1-x_0|\\
\end{align*}
$$

Since $0< C < 1$, we have that $0< 1-C^{m+1} < 1$ consequently $C^n\frac{1-C^{m+1}}{1-C} < \frac{C^n}{1-C}$.

Finally, $|x_m-x_n|<\frac{C^n}{1-C}|x_1-x_0|$ so for any $\epsilon > 0$ we can find sufficiently large $N$ such that $|x_m-x_n| < \epsilon$ for all $m,n > N$.

---
c)

First note that 
$$
\begin{align*}
    |f(x)-x| &< |f(x)-x_m|+|x_m-x|\\
    &=|f(x)-f(x_{m-1})|+|x_m-x|\\
    &\leq C|x-x_{m-1}|+|x_m-x|
\end{align*}
$$

Now by convergence of $(x_n)$, for any $\epsilon > 0$ we can find sufficiently large $N$ such that $C|x-x_{m-1}|+|x_m-x| < \epsilon$, which implies that $|f(x)-x| = 0 \implies f(x)=x$.

---
d)

Suppose that there is $y$ such that $f(y)=y$ and $y\neq x$. 

We have already proved that $(x_n) \to x$ which is a fixed point of $f$.

Note then that:
$$
    |x-y| = |f(x)-f(y)| \leq C|x-y|
$$

Consequently, $1 \leq C$ which is a contradiction, therefore $x=y$.

